# 

## 3

8 -12
10 -15

1 -3/2
1 -3/2

1 -3/2

## 4

$\begin{bmatrix}1 -3 2 -4\\0 1 5 5\\-3 11 4 22\end{bmatrix}$

$\begin{bmatrix}1 -3 2 -4\\0 1 5 5\\0 2 10 10\end{bmatrix}$

$\begin{bmatrix}1 -3 2 -4\\0 1 5 5\\0 0 0 0\end{bmatrix}$

## 8

$\begin{bmatrix}-3 9 6 | 0\\-3 9 -6.75+3/2k | 0\end{bmatrix}$

3/2k = 12.75
3k = 24.5
3k = 49/2
k = 49/6

i dont think i can do arithmetic

## 9

$\begin{bmatrix}-3 1.5 12\\3 -1.5 -20.5+k\end{bmatrix}$

$\begin{bmatrix}-3 1.5 12\\-3 1.5 20.5-k\end{bmatrix}$
12 = 20.5 - k
8.5 = k

## 12

$f(e_4) = [4 1] f(e_7) = [-5 -4] f(e_8) = [1 -1]$
f(2e_4) + f(3e_7) + f(-4e_8) + f(-6e_7)
f(2e_4) + f(-3e_7) + f(-4e_8)
[8 2] + [15 12] + [-4 4]
[19 18]

## 14

$\begin{bmatrix}1 1 0\\0 1 1\\1 0 1\end{bmatrix}$

$\begin{bmatrix}1 1 0\\0 1 1\\0 -1 1\end{bmatrix}$

$\begin{bmatrix}1 0 -1\\0 1 1\\0 0 1\end{bmatrix}$

$\begin{bmatrix}1 0 0\\0 1 0\\0 0 1\end{bmatrix}$

## 16

$\begin{bmatrix}{x - y - 1} -3 6\\3 {x - 4} -5\end{bmatrix}$
x-y-1 = 2
x-4 = 2x + y

x -y = 3
-x -y = 4

$\begin{bmatrix}1 -1 | 3\\-1 -1 | 4\end{bmatrix}$

$\begin{bmatrix}1 -1 | 3\\0 -2 | 7\end{bmatrix}$

$\begin{bmatrix}1 -1 | 3\\0 1 | -7/2\end{bmatrix}$

$\begin{bmatrix}1 0 | 3-\frac72\\0 1 | -7/2\end{bmatrix}$

6/2 - 7/2 = -1/2

## 17

$\begin{bmatrix}2 -4\\-9 0\end{bmatrix}\begin{bmatrix}-5 7\\9 -3\end{bmatrix}$
$\begin{bmatrix}-46 26\\45 -63\end{bmatrix}$

## 19

$A = \begin{bmatrix}-3 -2\\0 1\end{bmatrix}$

$A^3 = \begin{bmatrix}-3 -2\\0 1\end{bmatrix}\begin{bmatrix}-3 -2\\0 1\end{bmatrix}\begin{bmatrix}-3 -2\\0 1\end{bmatrix}$

$\begin{bmatrix}-3 -2\\0 1\end{bmatrix}\begin{bmatrix}-3 -2\\0 1\end{bmatrix}$
$\begin{bmatrix}9 4\\0 1\end{bmatrix}$

$A^3 = \begin{bmatrix}-3 -2\\0 1\end{bmatrix}\begin{bmatrix}9 4\\0 1\end{bmatrix}$
$\begin{bmatrix}-3 -2\\0 1\end{bmatrix}\begin{bmatrix}9 4\\0 1\end{bmatrix}$

$\begin{bmatrix}-27 -14\\0 1\end{bmatrix}$

$A^3 = \begin{bmatrix}-27 -14\\0 1\end{bmatrix}$

## 4 part 2

$\begin{bmatrix}1 -3 2 -4 | 0\\0 1 5 5 | 0\\-3 11 4 22 | 0\end{bmatrix}$

$\begin{bmatrix}1 -3 2 -4 | 0\\0 1 5 5 | 0\\0 2 -2 10 | 0\end{bmatrix}$

$\begin{bmatrix}1 0 17 11 | 0\\0 1 5 5 | 0\\0 0 -12 0 | 0\end{bmatrix}$

$\begin{bmatrix}1 0 0 11 | 0\\0 1 0 5 | 0\\0 0 1 0 | 0\end{bmatrix}$

$x_1 = -11x_4$
$x_2 = -5x_4$
$x_3 = 0$
$x_4 = x_4$

$\begin{bmatrix}1 -3 2 -4 | 0\\0 1 5 5 | 0\\1 -4 -3 -9 | 0\end{bmatrix}$

$\begin{bmatrix}1 -3 2 -4 | 0\\0 1 5 5 | 0\\0 -1 -5 -5 | 0\end{bmatrix}$

$\begin{bmatrix}1 -3 2 -4 | 0\\0 1 5 5 | 0\\0 0 0 0 | 0\end{bmatrix}$

$\begin{bmatrix}1 0 17 11 | 0\\0 1 5 5 | 0\\0 0 0 0 | 0\end{bmatrix}$

$x_1 = -17x_3 - 11x_4$
$x_2 = -5x_3 -5x_4$

